Include finTypes

CFG.v
@@ -9,14 +9,12 @@ Require Import Lists.List.
 Require Import Coq.Program.Equality.
 Require Import Coq.Program.Utils.
 
+(*Require Import finiteTypes.External.
+Require Import finiteTypes.BasicDefinitions.*)
+
+Require Import fin.FinTypes.
 
 Require Export Graph.
-
-(** basic parameters **)
-Parameter Lab : Type.
-Parameter Lab_dec : EqDec Lab eq.
-
-Hint Resolve Lab_dec.
 
 (*  Notation "p '-->*' q" := (exists π, Path p q π) (at level 55, right associativity).*)
 
@@ -25,7 +23,7 @@ Reserved Infix "-a>" (at level 55).
 Reserved Infix "-a>*" (at level 55).
 
 Class redCFG
-      (all_lab : list Lab)
+      (Lab : finType)
       (edge : Lab -> Lab -> bool)
       (root : Lab) 
       (a_edge : Lab -> Lab -> bool)
@@ -35,14 +33,12 @@ Class redCFG
                      where "p -->b q" := (edge p q);
       back_edge := (fun p q => back_edge_b p q = true)
                    where "p --> q"  := (p -->b q = true);
-      edge_incl1 : forall p q, p --> q -> p ∈ all_lab;
-      edge_incl2 : forall p q, p --> q -> q ∈ all_lab;
       loop_head_dom : forall ql qh, back_edge ql qh -> Dom edge root qh ql
       where "p -a> q" := (a_edge p q = true);
       a_edge_incl : sub_graph a_edge edge
       where "p '-a>*' q" := (exists π, Path a_edge p q π);
       a_edge_acyclic : acyclic a_edge;
-      reachability : forall q, q ∈ all_lab -> (exists π, Path edge root q π);
+      reachability : forall q, (exists π, Path edge root q π);
       loop_contains qh q := exists p π, back_edge p qh /\ Path edge q p π /\ (qh ∉ π \/ q = qh);
       exit_edge h p q := loop_contains h p /\ ~ loop_contains h q /\ p --> q;
       single_exit : forall h p q, exit_edge h p q -> forall h', exit_edge h' p q -> h = h';
@@ -51,32 +47,71 @@ Class redCFG
       (*no_head_split : forall h p q, loop_head h -> h --> p -> h --> q -> p = q*)
     }.
 
-Notation "p '-a>b' q" := ((fun (a_edge : Lab -> Lab -> bool)
-                             (_ : redCFG _ _ _ a_edge) => a_edge) _ _ p q)
+
+Notation "p '-a>b' q" := ((fun (Lab : finType)
+                             (a_edge : Lab -> Lab -> bool)
+                             (_ : redCFG Lab _ _ a_edge) => a_edge) _ _ _ p q)
                            (at level 55).
 
 Notation "p '-a>' q" := (p -a>b q = true) (at level 55).
 
-Infix "-->b" := ((fun (edge : Lab -> Lab -> bool)
-                    (_ : redCFG _ edge _ _) => edge)_ _) (at level 55).
+Notation "p '-->b' q" := ((fun (Lab : finType)
+                           (edge : Lab -> Lab -> bool)
+                           (root : Lab)
+                           (a_edge : Lab -> Lab -> bool)
+                           (_ : @redCFG Lab edge _ _) => edge) _ _ _ _ _ p q) (at level 55).
 
-Notation "p --> q" := (p -->b q = true) (at level 55, right associativity).
+Notation "p '-->' q" := (p -->b q = true) (at level 55, right associativity).
 
-Notation "p '-->*' q" := ((fun (edge : Lab -> Lab -> bool)
-                             (_ : redCFG _ edge _ _) => exists π, Path edge p q π) _ _)
+Notation "p '-->*' q" := ((fun (Lab : finType)
+                             (edge : Lab -> Lab -> bool)
+                             (root : Lab)
+                             (a_edge : Lab -> Lab -> bool)
+                             (_ : @redCFG Lab edge root a_edge)
+                             (p q : Lab)
+                           => exists π, Path edge p q π) _ _ _ _ _ p q)
                            (at level 55, right associativity).
 
-Notation "p '-a>*' q" := ((fun (a_edge : Lab -> Lab -> bool)
-                             (_ : redCFG _ _ _ a_edge)
-                           => exists π, Path a_edge p q π) _ _) (at level 55).
+Notation "p '-a>*' q" := ((fun (Lab : finType)
+                             (edge : Lab -> Lab -> bool)
+                             (root : Lab)
+                             (a_edge : Lab -> Lab -> bool)
+                             (_ : @redCFG Lab edge root a_edge)
+                             (p q : Lab)
+                           => exists π, Path a_edge p q π) _ _ _ _ _ p q) (at level 55).
 
 Infix "↪" := back_edge (at level 55).
+
+Local Ltac prove_spec :=
+  intros;
+  let tac :=
+      fun _ => lazymatch goal with
+              [ |- to_bool ?e = true <-> ?p] => destruct e; cbn; split; eauto ; intros; congruence
+            end
+  in
+  lazymatch goal with
+  | [ |- ?f _ _ _ = true <-> ?p ]
+    => unfold f; tac 0
+  | [ |- ?f _ _ = true <-> ?p ]
+    => unfold f; tac 0
+  | [ |- ?f _ = true <-> ?p ]
+    => unfold f; tac 0
+  | [ |- ?f = true <-> ?p ]
+    => unfold f; tac 0
+  end.
 
 Section red_cfg.
 
   Definition CPath `{redCFG} := Path edge.
 
   Context `{C : redCFG}.
+  
+  Instance Lab_dec : EqDec Lab eq.
+  Proof.
+    intros x y. destruct (decide_eq x y).
+    - left. rewrite e. reflexivity.
+    - right. eauto.
+  Qed.
 
   Definition CPath' π := CPath (ne_back π) (ne_front π) π.
 
@@ -91,31 +126,61 @@ Section red_cfg.
 
   (** decidable properties on redCFG **)
   
-  Lemma loop_head_dec p : {loop_head p} + {~ loop_head p}.
-  Admitted.
+  Lemma loop_head_dec p : dec (loop_head p).
+    eauto.
+  Qed.
 
-  Parameter loop_head_b : Lab -> bool.
-  Parameter loop_head_spec : forall p : Lab, loop_head_b p = true <-> loop_head p.
+  Definition loop_head_b p : bool := to_bool (loop_head_dec p).
+  Lemma loop_head_spec : forall p : Lab, loop_head_b p = true <-> loop_head p.
+    prove_spec.
+  Qed.
 
-  Lemma loop_contains_dec qh q : {loop_contains qh q} + {~ loop_contains qh q}.
+  Instance ne_list_eq_dec (A : Type) : eq_dec A -> eq_dec (ne_list A).
+  Proof.
+    intros H l.
+    induction l; intro l'; induction l'.
+    - decide (a = a0); subst;[left|right];eauto. contradict n. inversion n;eauto.
+    - right. intro N; inversion N.
+    - right. intro N; inversion N.
+    - decide (a = a0).
+      + subst. destruct (IHl l').
+        * subst. left. reflexivity.
+        * right. intro N; inversion N. congruence.
+      + right. intro N; inversion N. congruence.
+  Qed.
+
+  Definition EqNeList (X : eqType) := EqType (ne_list X).
+
+  Lemma loop_contains_dec qh q : dec (loop_contains qh q).
+    unfold loop_contains. eauto.
+    eapply finType_exists_dec. intros.
+    (* proof idea : consider only dupfree paths, there are only finitely many of them. *)
   Admitted.
+  Hint Resolve loop_contains_dec.
   
   Definition loop_contains_b qh q := to_bool (loop_contains_dec qh q).
 
-  Parameter loop_contains_spec : forall qh q, loop_contains_b qh q = true <-> loop_contains qh q.
-
-  (*  Definition loop_contains_spec `*)
+  Lemma loop_contains_spec : forall qh q, loop_contains_b qh q = true <-> loop_contains qh q.
+  Proof.
+    intros. unfold loop_contains_b. destruct (loop_contains_dec qh q); cbn; split;eauto.
+    intro. congruence.
+  Qed.
 
   Definition deq_loop q p : Prop :=
     forall h, loop_contains h p -> loop_contains h q.
 
-  Definition deq_loop_dec h p : {deq_loop h p} + {~ deq_loop h p}.
-  Admitted.
+  Instance deq_loop_dec h p : dec( deq_loop h p).
+    unfold deq_loop. eapply finType_forall_dec. intros.
+    eapply impl_dec; eapply loop_contains_dec.
+  Qed.
 
   Definition deq_loop_b h p
     := to_bool (deq_loop_dec h p).
-
-  Parameter deq_loop_spec : forall h p, deq_loop_b h p = true <-> deq_loop h p.
+  
+  Lemma deq_loop_spec : forall h p, deq_loop_b h p = true <-> deq_loop h p.  
+  Proof.
+    prove_spec.
+  Qed.
   
   Lemma deq_loop_refl l :
     deq_loop l l.
@@ -126,6 +191,7 @@ Section red_cfg.
   Lemma deq_loop_exited h qe e
         (Hexit : exit_edge h qe e)
     : deq_loop qe e.
+  Proof.
   Admitted.
   
   Lemma deq_loop_exiting h qe e
@@ -145,26 +211,64 @@ Section red_cfg.
         (Hloop : loop_contains h p)
     : deq_loop p h.
   Admitted.
-  
-  Definition innermost_loop h p : Prop := loop_head h /\ deq_loop h p /\ loop_contains h p.
 
-  Lemma ex_innermost_loop p
-    : p ∈ all_lab -> ~ deq_loop root p -> exists h, innermost_loop h p.
+  
+
+  Instance exit_edge_dec : forall h p q, dec (exit_edge h p q).
   Proof.
-    intros Hin N. unfold innermost_loop,deq_loop in *.
-    eapply reachability in Hin as [π Hπ].
+    intros; unfold exit_edge. eapply and_dec;[eauto| eapply and_dec];eauto. eapply not_dec. eauto.
+  Qed.
+  
+  Definition exit_edge_b h p q : bool := to_bool (exit_edge_dec h p q).
+  Lemma exit_edge_b_spec : forall h p q, exit_edge_b h p q = true <-> exit_edge h p q.
+  Proof.
+    prove_spec.
+  Qed.
+  
+  Instance decide_decPred_bool (A : Type) (f : A -> bool) a : dec (if f a then True else False).
+  Proof.
+    cbn. destruct (f a); eauto.
+  Qed.
+  
+  Definition decPred_bool (A : Type) (f : A -> bool) := DecPred (fun a => if f a then True else False).
+
+  Definition finType_sub_decPred (X : finType) (p : decPred X) : finType.
+  Proof.
+    eapply (@finType_sub X p). eapply decide_pred. 
+  Defined.
+
+  Definition finType_sub_bool (X : finType) (p : X -> bool) : finType.
+  Proof.
+    eapply (@finType_sub X (decPred_bool p)). eauto. Show Proof.
+  Defined.
+  
+  Definition depth (p : Lab) := Cardinality (finType_sub_bool (fun h => loop_contains_b h p)). 
+  
+  Definition innermost_loop h p : Prop :=  loop_contains h p /\ deq_loop h p.
+
+  Lemma strong_reachability q
+    : { π : ne_list Lab | Path edge root q π }.
+  Admitted.
+  
+  Lemma ex_innermost_loop p
+    : 0 < depth p -> { h : Lab | innermost_loop h p}.
+  Proof.
+    intros Hlt. unfold innermost_loop,deq_loop in *.
+    specialize (strong_reachability) as [π Hπ].
     (* pick last header, but not if it has an exit, in Hπ, exists because of N *)
   Admitted.
-
-  Parameter get_innermost_loop : Lab -> Lab.
-  Parameter get_innermost_loop_spec : forall p h, get_innermost_loop p = h <-> loop_contains h p /\ deq_loop h p.
-
-  Parameter exit_edge_b : forall `{redCFG}, Lab -> Lab -> Lab -> bool.
-  Parameter exit_edge_b_spec : forall h p q, exit_edge_b h p q = true <-> exit_edge h p q.
-
-  Parameter exit_edge_num : forall `{redCFG}, Lab -> Lab -> nat.
-
-  Definition depth p := length (filter (fun q => loop_contains_b q p) all_lab).
+  
+  Definition get_innermost_loop (p : Lab) : Lab.
+  Proof.
+    destruct (depth p) eqn:E.
+    - exact root.
+    - assert (0 < depth p) by omega. eapply ex_innermost_loop in H as [h H]. exact h.
+  Defined.
+  
+  Lemma get_innermost_loop_spec : forall p h, get_innermost_loop p = h <-> (depth p = 0 /\ h = root)
+                                                                    \/ (innermost_loop h p).
+  Proof.
+  Admitted.
 
   Definition exiting (h p : Lab) : Prop :=
     exists q, exit_edge h p q.
@@ -172,9 +276,15 @@ Section red_cfg.
   Definition exited (h q : Lab) : Prop :=
     exists p, exit_edge h p q.
 
-  Definition preds `{redCFG all_lab edge} p : list Lab := filter (fun q => edge q p) all_lab. 
+  Global Instance exited_dec (h q : Lab) : dec (exited h q).
+  Proof.
+    unfold exited. 
+    eapply finType_exists_dec; intros; eauto.
+  Qed.
 
-  Definition filter_loop h := filter (loop_contains_b h) all_lab.
+  Definition preds `{redCFG Lab edge} p : list Lab := filter (decPred_bool (fun q => edge q p)) (elem Lab). 
+
+  Definition filter_loop h := filter (decPred_bool (loop_contains_b h)) (elem Lab).
 
   Definition In_b {A : Type} `{H : EqDec A eq} (a : A) (l : list A)
     := if in_dec H a l then true else false.
@@ -185,10 +295,10 @@ Section red_cfg.
     intro Q. unfold loop_head, loop_contains in *. destruct Q as [p [_ [Q _]]].
     eexists; eauto.
   Qed.
-  
-  Lemma back_edge_incl p q : back_edge p q -> p --> q.
-  Proof.
-    unfold back_edge,back_edge_b. eapply minus_subgraph.
+
+  Lemma back_edge_incl (p q : Lab) (Hback : p ↪ q) : p --> q.
+  Proof. 
+    unfold back_edge,back_edge_b in Hback. eapply minus_subgraph. eauto.
   Qed.
 
   Lemma back_edge_dec p q : {p ↪ q} + {~ p ↪ q}.
@@ -201,42 +311,36 @@ Section red_cfg.
 
   (** simple propositions **)
 
-  Lemma path_in_alllab1 p q :
+(*  Lemma path_in_alllab1 p q :
     p <> q -> p -->* q -> p ∈ all_lab.
   Proof.
     intros Hneq Hpath.
     destruct Hpath. revert dependent q.
     induction x; intros q Hneq Hpath; inversion Hpath;[contradiction|subst].
-    decide' (p == b).
+    decide (p = b);subst.
     - eapply edge_incl1;eauto.
     - eapply IHx;eauto.
-  Qed.
+  Qed.*)
   
-  Lemma path_in_alllab2 p q :
+(*  Lemma path_in_alllab2 p q :
     p <> q -> p -->* q -> q ∈ all_lab.
   Proof.
     intros Hneq Hpath.
     destruct Hpath. inversion H; [contradiction|eapply edge_incl2;eauto].
-  Qed.
+  Qed.*)
   
   Lemma loop_reachs_member (h q : Lab)
-    : loop_contains h q ->h -->* q.
+    : loop_contains h q -> h -->* q.
   Proof.
     intros Hloop. unfold loop_contains in Hloop.
     destructH.
-    assert (q ∈ all_lab).
-    {
-      decide' (q == p).
-      - eapply edge_incl1. apply back_edge_incl;eauto.
-      - eapply path_in_alllab1;eauto.
-    }
     destruct Hloop3;[|subst q; eexists; econstructor].
-    eapply reachability in H. destructH. eapply loop_head_dom in Hloop0.
+    specialize (reachability q) as H'. destructH. eapply loop_head_dom in Hloop0.
     eapply path_app in Hloop2;eauto. eapply Hloop0 in Hloop2. eapply in_nl_conc in Hloop2.
     destruct Hloop2;[contradiction|].
     assert (h ∈ π0).
     { destruct π0; cbn in *;[contradiction|right;eauto]. }
-    eapply path_from_elem in H2;eauto. firstorder.
+    eapply path_from_elem in H1;eauto. firstorder. 
   Qed.
   
   Lemma dom_loop h
@@ -259,17 +363,11 @@ Section red_cfg.
     rewrite Q2 in H; cbn in H; congruence.
   Qed.
 
-  Lemma loop_head_in_graph h : loop_head h -> h ∈ all_lab.
-    intro Q.
-    unfold loop_head in *.  destructH.
-    eapply edge_incl2;eapply back_edge_incl;eauto.
-  Qed.
-
   Lemma dom_path p q
-    : q ∈ all_lab -> Dom edge root p q -> p -->* q.
+    : Dom edge root p q -> p -->* q.
   Proof.
-    intros Hin Hdom.
-    eapply reachability in Hin as [π Hπ]. specialize (Hdom π Hπ).
+    intros Hdom.
+    specialize reachability as [π Hπ]. specialize (Hdom π Hπ).
     eapply path_from_elem in Hπ; eauto using Lab_dec. firstorder.
   Qed.
 
@@ -301,12 +399,12 @@ Section red_cfg.
     : loop_contains h q -> ~ loop_contains h p -> Dom edge p h q.
   Proof.
     intros Hloop Hnloop.
-    decide' (p == q); [contradiction|].
+    decide (p = q); [subst;contradiction|].
     unfold loop_contains in Hloop. destructH.
     destruct Hloop3 as [Hloop3|Hloop3];[|subst q;eapply dominant_self]. rename π into π1.
     intros π Hπ.
-    assert (p ∈ all_lab) as H0 by (eapply path_in_alllab1;eauto).
-    eapply reachability in H0. destructH.
+(*    assert (p ∈ all_lab) as H0 by (eapply path_in_alllab1;eauto).*)
+    specialize reachability as Hϕ.
     unfold loop_contains in Hnloop.
     rewrite DM_not_exists in Hnloop. setoid_rewrite DM_not_exists in Hnloop.
     eapply path_app in Hloop2;eauto.
@@ -327,12 +425,10 @@ Section red_cfg.
     intros Hl. unfold loop_contains.
     - unfold loop_head in Hl. destruct Hl. 
       eapply loop_head_dom in H as Hdom.
-      eapply back_edge_incl in H as Hreach. specialize (reachability x) as Hreach'.
-      exploit' Hreach'.
-      + eapply edge_incl1;eauto.
-      + destructH.
-        eapply Hdom in Hreach' as Hreach''. eapply path_from_elem in Hreach'; eauto.
-        destructH; eauto. eexists; eexists. firstorder; eauto.
+      eapply back_edge_incl in H as Hreach. specialize (@reachability _ _ _ _ _ x) as Hreach'.
+      destructH.
+      eapply Hdom in Hreach' as Hreach''. eapply path_from_elem in Hreach'; eauto.
+      destructH; eauto. eexists; eexists. firstorder; eauto.
   Qed.
   
   Lemma NoDup_rcons (A : Type) (x : A) (l : list A)
@@ -361,7 +457,7 @@ Section red_cfg.
     : CPath h q π -> loop_contains h q -> NoDup π -> forall p, p ∈ π -> loop_contains h p.
   Proof.
     intros Hπ Hin Hnd p Hp. 
-    destruct (p == h) as [Hph|Hph].
+    decide (p = h) as [Hph|Hph].
     - rewrite Hph. eapply loop_contains_self. eapply loop_contains_loop_head; eauto.
     - destruct (loop_contains_dec h p) as [N|N]; [eauto|exfalso].
       eapply path_from_elem in Hp; eauto. destructH.
@@ -422,26 +518,111 @@ Section red_cfg.
     : loop_contains h p -> p ↪ h' -> loop_contains h h'.
   Proof.
   Admitted.
+  
+  Definition finType_sub_elem (h : Lab) (p : decPred Lab) : p h -> finType_sub_decPred p.
+    intros H.
+    econstructor. unfold pure. instantiate (1 := h). decide (p h);eauto.
+  Defined.
 
-  Program Instance loop_CFG
-          (h : Lab)
-    : redCFG (filter (fun p => loop_contains_b h p) all_lab)
-             (edge ∩ loop_edge h)
-             h
-             (a_edge ∩ loop_edge h).
-  Next Obligation.
-    eapply filter_In.
+  Open Scope prg.
+
+  Definition restrict_edge (f : Lab -> Lab -> bool) (p : decPred Lab)
+    : let L' := finType_sub_decPred p in L' -> L' -> bool
+    := fun x y => (f (`x) (`y)).
+
+  Definition loop_edge_dp (h : Lab) := decPred_bool (fun p => loop_contains_b h p).
+
+  Lemma loop_edge_h_invariant (h : Lab) (H : loop_head h) : loop_edge_dp h h.
+  Proof.
+    unfold loop_edge_dp. cbn. destruct (loop_contains_b h h) eqn:E;[exact I|].
+    rewrite <-not_true_iff_false in E. eapply E.
+    rewrite loop_contains_spec. now eapply loop_contains_self.
+  Qed.
+
+End red_cfg.
+
+Arguments finType_sub_elem {_}.
+Arguments restrict_edge {_}.
+
+(** * sub_CFG **)
+
+Program Instance sub_CFG
+        `{C : redCFG}
+        (P : decPred Lab)
+        (r : Lab)
+        (HP : P r)
+        (Hloop : forall p, P p -> loop_contains r p \/ r = root)
+        (Hreach : forall p, exists π, Path (restrict_edge edge P)
+                                            (finType_sub_elem r P HP) 
+                                            p π)
+  : @redCFG (finType_sub_decPred P)
+            (restrict_edge edge P)
+            (finType_sub_elem r P HP)
+            (restrict_edge a_edge P).
+
+Next Obligation. (* loop_head_dom *)
+  (* eapply dom_intersection,loop_head_dom,minus_back_edge;eauto. *)
+Admitted.
+Next Obligation. (* a_edge_incl *)
+  (* eapply intersection2_subgraph; apply a_edge_incl.*)
+Admitted.
+Next Obligation. (* a_edge_acyclic *)
+  eapply acyclic_subgraph_acyclic.
+  - admit. (*eapply intersection_subgraph1.*)
+  - eapply a_edge_acyclic.
+    Unshelve. all:eauto.
+Admitted.
+Next Obligation. (* single_exit *)
+  destruct h; destruct h'. destruct H12, H8.
+  - admit.
+  - admit.
+  - admit.
+  - rewrite <-H12. rewrite <-H8. reflexivity.
+Admitted.
+Next Obligation. (* no_head_exit *)
+Admitted.
+
+(** * loop_CFG **)
+
+Instance loop_CFG
+           `{C : redCFG}
+           (h : Lab)
+           (H : loop_head h)
+  : @redCFG (finType_sub_decPred (loop_edge_dp h))
+            (restrict_edge edge (loop_edge_dp h))
+            (finType_sub_elem h (loop_edge_dp h) (loop_edge_h_invariant H))
+            (restrict_edge a_edge (loop_edge_dp h)).
+Proof.
+  eapply sub_CFG; intros.
+  - left. unfold loop_edge_dp in H0. cbn in H0. destruct (loop_contains_b h p) eqn:E;[|contradiction].
+    eapply loop_contains_spec;eauto.
+  - admit.
+Admitted.
+
+(*
+
+Program Instance loop_CFG
+        `{C : redCFG}
+        (h : Lab)
+        (H : loop_head h)
+  : @redCFG (finType_sub_decPred (loop_edge_dp h))
+            (restrict_edge (edge ∩ loop_edge h) (loop_edge_dp h))
+            (finType_sub_elem h (loop_edge_dp h) (loop_edge_h_invariant H))
+            (restrict_edge (a_edge ∩ loop_edge h) (loop_edge_dp h)).
+(*  Next Obligation.
+    eapply in_filter_iff.
     split; [eapply intersection_subgraph1 in H|eapply intersection_subgraph2 in H].
     - eapply edge_incl1;eauto.
-    - unfold loop_edge in H. eapply intersection_subgraph1 in H. eapply H.
+    - unfold loop_edge in H. eapply intersection_subgraph1 in H. unfold decPred_bool. cbn. rewrite H. exact I.
   Qed.
   Next Obligation.
-    eapply filter_In.
+    eapply in_filter_iff.
     split; [eapply intersection_subgraph1 in H|eapply intersection_subgraph2 in H].
     - eapply edge_incl2;eauto.
-    - unfold loop_edge in H. eapply intersection_subgraph2 in H. eapply H.
-  Qed.
-  Next Obligation.
+    - unfold loop_edge in H. eapply intersection_subgraph2 in H. cbn. rewrite H. exact I.
+  Qed.*)
+Next Obligation. (* loop_head_dom *)
+Admitted. (*
     destruct (loop_head_dec h) as [H0|H0];[|admit].
     eapply dom_intersection.
     eapply dom_trans ; eauto.
@@ -453,79 +634,73 @@ Section red_cfg.
         eapply intersection_subgraph1 in H; eapply loop_contains_spec;eauto.
       + eapply minus_back_edge;eauto. 
     - eapply loop_head_dom. eapply minus_back_edge; eauto.
-  Admitted.
-  Next Obligation.
-    eapply intersection2_subgraph; apply a_edge_incl.
-  Qed.
-  Next Obligation.
-    eapply acyclic_subgraph_acyclic.
-    - eapply intersection_subgraph1.
-    - eapply a_edge_acyclic.
-  Qed.
+  Admitted.*)
+Next Obligation. (* subgraph *)
+  eapply intersection2_subgraph. eapply a_edge_incl.
 
+Admitted.
+Next Obligation. (* acyclic *)
+  eapply acyclic_subgraph_acyclic.
+  - eapply intersection_subgraph1.
+  - eapply a_edge_acyclic.
+Admitted.
+
+(*
   Lemma loop_contains_in_alllab h p :
     loop_contains h p -> p ∈ all_lab.
   Proof.
     intros Hloop. destruct Hloop. destructH.
-    decide' (x == p).
+    decide (x = p);subst.
     - eapply edge_incl1; eapply back_edge_incl; eauto.
     - eapply path_in_alllab1;eauto.
-  Qed.
+  Qed.*)
 
-  Lemma loop_edge_reach_help h p (*q*)
+(*  Lemma loop_edge_reach_help `{C : redCFG} h p (*q*)
         (Hhead : loop_head h)
         (*        (Hedge : (edge ∩ loop_edge h) p q = true)*)
         (Hloop : loop_contains h p)
     : exists π, Path (edge ∩ loop_edge h) h p π.
   Proof.
-    assert (p ∈ all_lab) as Hin by (eapply loop_contains_in_alllab;eauto).
-    eapply dom_path with (p:=h) in Hin as [π Hπ];[|eapply dom_loop;eauto].
+    (*assert (p ∈ all_lab) as Hin by (eapply loop_contains_in_alllab;eauto).*) (* TODO *)
+    specialize (dom_path h) as [π Hπ];[|eapply dom_loop;eauto].
+    assert (EqDec Lab eq) as HHeq by eauto.
     specialize (path_NoDup _ _ _ _ _ (ex_intro _ π Hπ)) as [φ [Hφ Hnd]].
     exists φ. eapply path_loop_edge;eauto. eapply loop_contains_path; eauto.
-  Qed.
-  
-  Next Obligation.
-    eapply filter_In in H. destructH.
+  Qed. *)
+
+Next Obligation. (* reachability *)
+(*
+    eapply in_filter_iff in H. destructH.
     destruct (loop_head_dec h) as [H|H];[|admit].
-    eapply loop_edge_reach_help;eauto;eapply loop_contains_spec;eauto.
-  Admitted.
-  Next Obligation.
-    (* since the original has single exits intersecting doesn't change anything *)
-  Admitted.
-  Next Obligation.
-    (* there are neither new heads nor new edges -> property follows *)
-  Admitted.  
+    eapply loop_edge_reach_help;eauto;eapply loop_contains_spec;eauto.*)
+Admitted.
+Next Obligation. (* single_exit *)
+  (* since the original has single exits intersecting doesn't change anything *)
+Admitted.
+Next Obligation. (* no_head_exit *)
+  (* there are neither new heads nor new edges -> property follows *)
+Admitted.  
+*)
 
-  Definition top_level `{redCFG} q := forall h, loop_contains h q -> (h = root \/ h = q).
-  
-  Parameter exit_edge_dec : forall `{redCFG} h q p, 
-      {exit_edge h p q} + {~ exit_edge h p q}.
-
-End red_cfg.
+Definition top_level `{redCFG} q := forall h, loop_contains h q -> (h = root \/ h = q).
 
 Arguments loop_CFG {_ _ _ _} (_).
 
-Definition head_exits_edge `{redCFG} :=
-  (fun h q
-   => to_bool (Exists_dec (fun p => exit_edge h p q)
-                         all_lab
-                         (exit_edge_dec h q))).
+(** * head_exits **)
 
-Parameter head_exits_edge_spec :
+Definition head_exits_edge `{redCFG} h q : bool
+  := if decision (exited h q) then true else false. 
+
+Lemma head_exits_edge_spec :
   forall `{redCFG} h q, head_exits_edge h q = true <-> exists p, exit_edge h p q.
+Proof.
+  intros. unfold head_exits_edge. decide (exited h q); split;cbn;eauto.
+  intros;congruence.
+Qed.
 
 Program Instance head_exits_CFG `(redCFG)
-  : redCFG all_lab (edge ∪ head_exits_edge) root (a_edge ∪ head_exits_edge).
-Next Obligation.
-  unfold union_edge in H0. conv_bool. destruct H0;[eapply edge_incl1|];eauto.
-  eapply head_exits_edge_spec in H0. destructH. unfold exit_edge in H0. destructH.
-  unfold loop_contains in H1. destructH. eapply edge_incl2;eapply back_edge_incl;eauto.
-Qed.
-Next Obligation.
-  unfold union_edge in H0. conv_bool. destruct H0;[eapply edge_incl2|];eauto.
-  eapply head_exits_edge_spec in H0. destructH. unfold exit_edge in H0.
-  eapply edge_incl2;destructH;eauto.
-Qed.
+  : redCFG (edge ∪ head_exits_edge) root (a_edge ∪ head_exits_edge).
+
 
 Lemma head_exits_in_path_head_incl `{redCFG} ql π
       (Hpath : Path (edge ∪ head_exits_edge) root ql π)
@@ -535,14 +710,14 @@ Admitted.
 Lemma head_exits_back_edge `{redCFG} ql qh :
   ((edge ∪ head_exits_edge) ∖ (a_edge ∪ head_exits_edge)) ql qh = true <-> ql ↪ qh.
 Admitted.
-Next Obligation.
+
+Next Obligation. (* loop_head_dom *)
   unfold Dom. intros π Hpath.
   rewrite head_exits_back_edge in H0.
   eapply head_exits_in_path_head_incl in Hpath. destructH. unfold loop_head in Hpath1.
   eapply loop_head_dom in Hpath0;eauto.
 Qed.
-
-Next Obligation.
+Next Obligation. (* a_edge_incl *)
   eapply union_subgraph.
   - exact a_edge_incl.
   - firstorder.
@@ -560,7 +735,7 @@ Lemma head_exits_same_connected `{redCFG} p q π
       (Hpath : Path (a_edge ∪ head_exits_edge) p q π)
   : exists ϕ, Path a_edge p q ϕ.
 Admitted.
-Next Obligation.
+Next Obligation. (* a_edge_acyclic *)
   unfold acyclic. intros p q Hedge [π Hπ]. eapply head_exits_same_connected in Hπ. destructH.
   unfold union_edge in Hedge; conv_bool. destruct Hedge as [Hedge|Hedge].
   - eapply a_edge_acyclic; eauto.
@@ -568,19 +743,19 @@ Next Obligation.
     eapply head_exits_path in Hedge. destructH. eapply path_path_acyclic;eauto.
     exact a_edge_acyclic.
 Qed.
-Next Obligation.
-  eapply reachability in H0. eapply subgraph_path in H0;eauto.
+
+Next Obligation. (* reachability *)
+  specialize reachability as H0. eapply subgraph_path in H0;eauto.
   unfold sub_graph,union_edge. firstorder.
 Qed.
-Next Obligation.
+Next Obligation. (* single_exit *)
   (* new exits don't have new targets, and the source has the same depth *)
 Admitted.
-Next Obligation.
+Next Obligation. (* no_head_exit *)
   (* new exits don't have new targets *)
 Admitted.
 
-
-Definition head_exits_property `(C : redCFG) := forall h p q, exit_edge h p q -> h --> q.
+Definition head_exits_property `(C : redCFG) := forall h p q, exit_edge h p q -> edge h q = true.
 
 Arguments exit_edge {_ _ _ _} (_).
 
@@ -598,39 +773,34 @@ Arguments exit_edge {_ _ _ _ _}.
 
 (** implode CFG **)
 (* assuming no exit-to-heads *)
-Definition implode_edge `{redCFG} := (fun p q => deq_loop_b root p && deq_loop_b root q
-                                              || deq_loop_b root p && loop_head_b q
-                                              || loop_head_b p && deq_loop_b root q).
 
-Program Instance implode_CFG `(H : redCFG) (Hhe : head_exits_property H)
-  : redCFG (filter (fun p => deq_loop_b root p
-                          || (depth p ==b S (depth root)) && loop_head_b p) all_lab)
-           (edge ∩ implode_edge)
-           root
-           (a_edge ∩ implode_edge).
-Next Obligation.
-  eapply filter_In.
-  split; [eapply intersection_subgraph1 in H0|eapply intersection_subgraph2 in H0].
-  - eapply edge_incl1;eauto.
-  - unfold implode_edge in H0. conv_bool. repeat destruct H0; eauto 2. admit.
+(*Definition implode_edge `{redCFG} := (fun p q => deq_loop_b root p && deq_loop_b root q
+                                              || deq_loop_b root p && loop_head_b q
+                                              || loop_head_b p && deq_loop_b root q).*)
+Definition implode_nodes `{C : redCFG}
+  := decPred_bool (fun p => deq_loop_b root p
+                         || (depth p ==b S (depth root)) && loop_head_b p).
+
+Lemma implode_nodes_root_inv `{C : redCFG}
+  : implode_nodes root.
+Proof.
+  unfold implode_nodes. cbn.
+  assert (deq_loop_b root root = true) as H.
+  {
+    rewrite deq_loop_spec. unfold deq_loop. firstorder.
+  }
+  rewrite H. cbn. exact I.
+Qed.      
+
+Instance implode_CFG `(H : redCFG) (Hhe : head_exits_property H)
+  : @redCFG (finType_sub_decPred implode_nodes)
+            (restrict_edge edge implode_nodes)
+            (finType_sub_elem root implode_nodes (implode_nodes_root_inv))
+            (restrict_edge a_edge implode_nodes).
+Proof.
+  eapply sub_CFG;intros;[eauto|].
 Admitted.
-Next Obligation.
-  eapply filter_In.
-  split; [eapply intersection_subgraph1 in H0|eapply intersection_subgraph2 in H0].
-  - eapply edge_incl2;eauto.
-  - unfold implode_edge in H0. conv_bool. repeat destruct H0; eauto 2.  admit.
-Admitted.
-Next Obligation.
-  eapply dom_intersection,loop_head_dom,minus_back_edge;eauto.
-Qed.
-Next Obligation.
-  eapply intersection2_subgraph; apply a_edge_incl.
-Qed.
-Next Obligation.
-  eapply acyclic_subgraph_acyclic.
-  - eapply intersection_subgraph1.
-  - eapply a_edge_acyclic.
-Qed.
+  
 
 Lemma prefix_induction {A : Type} {P : list A -> Prop}
   : P nil
@@ -650,6 +820,7 @@ Proof.
   - admit.
 Admitted.
 
+(*
 Next Obligation.
   eapply filter_In in H0. destructH. eapply reachability in H1. destruct H1 as [π Hπ].
   conv_bool. rewrite deq_loop_spec in H2.
@@ -686,24 +857,27 @@ Next Obligation.
          } 
          unfold innermost_loop in E. destructH.
          admit.
-Admitted.
-Next Obligation.
-  (* as in loop_edge_CFG *)
-Admitted.
-Next Obligation.
-  (* as in loop_edge_CFG *)
-Admitted.
+Admitted.*)
 
-Definition local_impl_CFG `(C : redCFG) (h : Lab) :=
-  let D := (loop_CFG C h) in 
-  implode_CFG (head_exits_CFG D) (head_exits_property_satisfied D).
+Definition local_impl_CFG `(C : redCFG) (h : Lab) : exists Lab' edge' root' a_edge',
+    @redCFG Lab' edge' root' a_edge'.
+Proof.
+  decide (loop_head h).
+  - specialize (loop_CFG C h l) as C1.
+    specialize (head_exits_CFG C1) as C2.
+    specialize (implode_CFG C2 (@head_exits_property_satisfied _ _ _ _ C1)) as C3.
+    do 4 eexists. eapply C3.
+  - specialize (head_exits_CFG C) as C2.
+    specialize (implode_CFG C2 (@head_exits_property_satisfied _ _ _ _ C)) as C3.
+    do 4 eexists. eapply C3.
+Defined.
 
 
 (** more parameters **)
 
-Lemma Lab_dec' : forall (l l' : Lab), { l = l' } + { l <> l'}.
+Lemma Lab_dec' `{redCFG} : forall (l l' : Lab), { l = l' } + { l <> l'}.
 Proof.
   apply Lab_dec.
 Qed.
 
-Parameter no_self_loops : forall `(C : redCFG), forall q p, q --> p -> q =/= p.
+Parameter no_self_loops : forall `(C : redCFG), forall q p, edge q p = true -> q =/= p.
